spc/SRF.v
@@ -1,0 +1,183 @@
+From stdpp Require Import coPset gmap namespaces.
+From sflib Require Import sflib.
+From iris Require Import bi.big_op.
+From iris Require base_logic.lib.invariants.
+From Coq Require Import Program Arith.
+Require Import Coqlib PCM PCMAux IProp IPM.
+
+Local Notation level := nat.
+
+Module PF.
+  
+  Class t: Type := {
+    shp: Type;
+    deg: shp -> forall (Prev:Type), Type;
+   }.
+
+End PF.
+
+Coercion PF.shp: PF.t >-> Sortclass.
+
+Module GPF.
+  
+  Class t: Type := __GATOM: nat -> PF.t.
+
+  Class inG (F: PF.t) (GF: t) : Type := {
+    inG_id: nat;
+    inG_prf: F = GF inG_id;
+  }.
+
+End GPF.
+
+Module SRFMSynG.
+  
+  Class t: Type := __GATM: GPF.t.
+
+End SRFMSynG.
+
+Module SRFSyn.
+
+  Section SYNTAX.
+
+  Context `{α: SRFMSynG.t}.
+
+  Inductive cons {Prev: Type} : Type :=
+  | lift (p: Prev) : cons
+  | _cur i (s: α i) (c: PF.deg s Prev -> cons)
+  .
+
+  Fixpoint _t (n : level) : Type :=
+    match n with
+    | O => Empty_set
+    | S m => cons (Prev:=_t m) 
+    end.
+
+  Definition t (n : level) : Type := _t (S n).
+
+  Fixpoint liftn n {m} (p: t m) : t (n+m) :=
+    match n return t (n+m) with
+    | 0 => p
+    | S n' => lift (liftn n' p)
+    end.
+  
+  End SYNTAX.
+
+End SRFSyn.
+
+Module SRFDom.
+
+  Class t : Type := {
+      dom: Type;
+      void: dom;
+    }.
+
+End SRFDom.
+
+Module SRFMSem.
+
+  Section SEM.
+
+  Context `{Δ: SRFDom.t}.
+  Context `{α: SRFMSynG.t}.
+  Context `{A: PF.t}.
+
+  Class t : Type := 
+    sem: forall n (s: A) (p: PF.deg s (SRFSyn._t n) -> SRFSyn.t n) (P: PF.deg s (SRFSyn._t n) -> SRFDom.dom), SRFDom.dom
+  .
+
+  End SEM.
+  
+End SRFMSem.
+
+Module SRFMSemG.
+
+  Section GSEM.
+
+  Context `{Δ: SRFDom.t}.
+    
+  Class t `{α: SRFMSynG.t}: Type := msem : forall i, SRFMSem.t (A:= α i).
+
+  Class inG (A: PF.t) (α: SRFMSynG.t) (B: @SRFMSem.t _ α A) (β: t) : Type := {
+    inG_id: nat;
+    inG_prf: existT A B = existT (α inG_id) (β inG_id);
+  }.
+  
+  End GSEM.
+
+End SRFMSemG.
+
+Module SRFSem.
+
+  Section SEM.
+
+  Context `{β: @SRFMSemG.t Δ α}.
+
+  Fixpoint _t n : SRFSyn._t n -> SRFDom.dom :=
+    match n with
+    | O => fun _ => SRFDom.void
+    | S m => fix _t_aux (syn : SRFSyn._t (S m)) : SRFDom.dom :=
+      match syn with
+      | SRFSyn.lift p => _t m p
+      | SRFSyn._cur i s c => β i m s c (_t_aux ∘ c)
+      end
+    end.
+
+  Definition t n : SRFSyn.t n -> SRFDom.dom := _t (S n).
+
+  Program Definition cur `{IN: @SRFMSemG.inG _ A α B β} {n} (c: {s: A & (PF.deg s (SRFSyn._t n) -> SRFSyn.t n)}) : SRFSyn.t n.
+    destruct c as [s c]. destruct IN. inv inG_prf.
+    exact (SRFSyn._cur inG_id s c).
+  Defined.
+  
+  End SEM.
+  
+End SRFSem.
+
+Module SRFRed.
+  
+  Section RED.
+
+  Context `{β: @SRFMSemG.t Δ α}.
+
+  Lemma cur `{IN: @SRFMSemG.inG _ A α B β} n s c :
+    SRFSem.t n (SRFSem.cur (existT s c)) = B _ s c (SRFSem.t n ∘ c).
+  Proof.
+    destruct IN eqn: EQ. subst. depdes inG_prf. ss.
+  Qed.
+
+  Lemma lift_0 c :
+    SRFSem.t 0 (SRFSyn.lift c) = SRFDom.void.
+  Proof. reflexivity. Qed.
+
+  Lemma lift n c :
+    SRFSem.t (S n) (SRFSyn.lift c) = SRFSem.t n c.
+  Proof. reflexivity. Qed.
+
+  End RED.
+
+End SRFRed.  
+
+Global Opaque SRFSem.cur.
+Global Opaque SRFSem.t.
+
+(** Notations *)
+
+Declare Scope SRF_scope.
+Delimit Scope SRF_scope with SRF.
+Bind Scope SRF_scope with SRFSyn.t.
+
+Local Open Scope SRF_scope.
+
+Notation "'⟨' A '⟩'" := (SRFSem.cur A) : SRF_scope.
+Notation "⤉ P" := (SRFSyn.lift P) (at level 20) : SRF_scope.
+(* Simple reduction tactics. *)
+
+Ltac SRF_red := (try rewrite ! @SRFRed.cur;
+                 try rewrite ! @SRFRed.lift_0;
+                 try rewrite ! @SRFRed.lift
+                ).
+
+Ltac SRF_red_all := (try rewrite ! @SRFRed.cur in *;
+                     try rewrite ! @SRFRed.lift_0 in *;
+                     try rewrite ! @SRFRed.lift in *
+                    ).
